demo/owned_heap/BoxTarget.v
@@ -3,19 +3,25 @@ From Coq Require Import String List ZArith.
 From compcert Require Import Coqlib Integers Floats AST Ctypes Cop Clight Clightdefs.
 Local Open Scope Z_scope.
 
-Definition _get : ident := 56%positive.
-Definition _key : ident := 54%positive.
-Definition _main : ident := 59%positive.
+
+Definition _delete : ident := 61%positive.
+Definition _fini : ident := 63%positive.
+Definition _free : ident := 54%positive.
+Definition _get : ident := 58%positive.
+Definition _init : ident := 62%positive.
+Definition _key : ident := 56%positive.
+Definition _main : ident := 64%positive.
 Definition _malloc : ident := 53%positive.
-Definition _new : ident := 55%positive.
-Definition _set : ident := 58%positive.
-Definition _val : ident := 57%positive.
-Definition _t'1 : ident := 60%positive.
+Definition _new : ident := 57%positive.
+Definition _set : ident := 60%positive.
+Definition _v : ident := 55%positive.
+Definition _val : ident := 59%positive.
+Definition _t'1 : ident := 65%positive.
 
 Definition f_new := {|
-  fn_return := (tptr tint);
+  fn_return := (tptr tvoid);
   fn_callconv := cc_default;
-  fn_params := nil;
+  fn_params := ((_v, tint) :: nil);
   fn_vars := nil;
   fn_temps := ((_key, (tptr tint)) :: (_t'1, (tptr tvoid)) :: nil);
   fn_body :=
@@ -26,29 +32,61 @@ Definition f_new := {|
       ((Esizeof tint tulong) :: nil))
     (Sset _key (Etempvar _t'1 (tptr tvoid))))
   (Ssequence
-    (Sassign (Ederef (Etempvar _key (tptr tint)) tint)
-      (Econst_int (Int.repr 0) tint))
+    (Sassign (Ederef (Etempvar _key (tptr tint)) tint) (Etempvar _v tint))
     (Sreturn (Some (Etempvar _key (tptr tint))))))
 |}.
 
 Definition f_get := {|
   fn_return := tint;
   fn_callconv := cc_default;
-  fn_params := ((_key, (tptr tint)) :: nil);
+  fn_params := ((_key, (tptr tvoid)) :: nil);
   fn_vars := nil;
   fn_temps := nil;
   fn_body :=
-(Sreturn (Some (Ederef (Etempvar _key (tptr tint)) tint)))
+(Sreturn (Some (Ederef (Ecast (Etempvar _key (tptr tvoid)) (tptr tint)) tint)))
 |}.
 
 Definition f_set := {|
   fn_return := tvoid;
   fn_callconv := cc_default;
-  fn_params := ((_key, (tptr tint)) :: (_val, tint) :: nil);
+  fn_params := ((_key, (tptr tvoid)) :: (_val, tint) :: nil);
   fn_vars := nil;
   fn_temps := nil;
   fn_body :=
-(Sassign (Ederef (Etempvar _key (tptr tint)) tint) (Etempvar _val tint))
+(Sassign (Ederef (Ecast (Etempvar _key (tptr tvoid)) (tptr tint)) tint)
+  (Etempvar _val tint))
+|}.
+
+Definition f_delete := {|
+  fn_return := tvoid;
+  fn_callconv := cc_default;
+  fn_params := ((_key, (tptr tvoid)) :: nil);
+  fn_vars := nil;
+  fn_temps := nil;
+  fn_body :=
+(Scall None
+  (Evar _free (Tfunction (Tcons (tptr tvoid) Tnil) tvoid cc_default))
+  ((Etempvar _key (tptr tvoid)) :: nil))
+|}.
+
+Definition f_init := {|
+  fn_return := tvoid;
+  fn_callconv := cc_default;
+  fn_params := ((_key, (tptr tvoid)) :: nil);
+  fn_vars := nil;
+  fn_temps := nil;
+  fn_body :=
+Sskip
+|}.
+
+Definition f_fini := {|
+  fn_return := tvoid;
+  fn_callconv := cc_default;
+  fn_params := ((_key, (tptr tvoid)) :: nil);
+  fn_vars := nil;
+  fn_temps := nil;
+  fn_body :=
+Sskip
 |}.
 
 Definition composites : list composite_definition :=
@@ -57,11 +95,13 @@ nil.
 Definition global_definitions : list (ident * globdef fundef type) :=
 ((_malloc,
    Gfun(External EF_malloc (Tcons tulong Tnil) (tptr tvoid) cc_default)) ::
+ (_free, Gfun(External EF_free (Tcons (tptr tvoid) Tnil) tvoid cc_default)) ::
  (_new, Gfun(Internal f_new)) :: (_get, Gfun(Internal f_get)) ::
- (_set, Gfun(Internal f_set)) :: nil).
+ (_set, Gfun(Internal f_set)) :: (_delete, Gfun(Internal f_delete)) ::
+ (_init, Gfun(Internal f_init)) :: (_fini, Gfun(Internal f_fini)) :: nil).
 
 Definition public_idents : list ident :=
-(_set :: _get :: _new :: _malloc :: nil).
+(_fini :: _init :: _delete :: _set :: _get :: _new :: _free :: _malloc :: nil).
 
 Definition prog : Clight.program := 
   mkprogram composites global_definitions public_idents _main Logic.I.
